Add locally nameless STLC

Play.v
@@ -1,18 +1,23 @@
 From Stdlib Require Import Arith.Arith.
 From Stdlib Require Import Strings.String.
 Require Import Coq.Unicode.Utf8.
+From TLC Require Import LibLN.
 
 Inductive term : Type :=
-  | bvar (i : nat) (* bound var *)
-  | fvar (x : nat) (* free var *)
-  | app (lhs : term) (rhs : term)
-  | lam (body : term).
+  | term_bvar (i : nat) (* bound var *)
+  | term_fvar (x : var) (* free var *)
+  | term_app (lhs : term) (rhs : term)
+  | term_lam (body : term).
 
 Inductive type : Type :=
-  | ftvar (x : nat) (* free type variable *)
-  | tfun (arg : type) (res : type).
+  | type_fvar (x : var) (* free type variable *)
+  | type_fun (arg : type) (res : type).
 
-Declare Custom Entry mylang.
+Coercion term_bvar : nat >-> term.
+Coercion term_fvar : var >-> term.
+Coercion type_fvar : var >-> type.
+
+(* Declare Custom Entry mylang.
 Notation "<{ e }>" := e (e custom mylang at level 99).
 Notation "( x )" := x (in custom mylang, x at level 99).
 Notation "'\f' ( A1 , .. , An ) -> T" := (tfun (cons A1 .. (cons An nil) ..) T) 
@@ -22,11 +27,199 @@ Notation "'\f' ( A1 , .. , An ) -> T" := (tfun (cons A1 .. (cons An nil) ..) T)
     right associativity).
 (* Coercion ftvar : nat >-> type. *)
 
-Example term0 : type := <{ \f ( (ftvar 1) ) -> (ftvar 3) }>.
+Example term0 : type := <{ \f ( (ftvar 1) ) -> (ftvar 3) }>. *)
+
+Fixpoint open_rec (k : nat) (u : term) (t : term) : term :=
+  match t with
+  | term_bvar i => if Nat.eqb k i then u else t
+  | term_fvar x => t
+  | term_app lhs rhs => term_app (open_rec k u lhs) (open_rec k u rhs)
+  | term_lam body => term_lam (open_rec (S k) u body)
+  end.
+
+Definition open t u := open_rec 0 u t.
+
+Notation "{ k ~> u } t" := (open_rec k u t) (at level 67).
+Notation "t ^^ u" := (open t u) (at level 67).
+Notation "t ^ x" := (open t (term_fvar x)).
+
+Inductive is_term : term -> Prop :=
+  | is_term_var : forall x,
+      is_term (term_fvar x)
+  | is_term_lam : forall L t,
+      (forall x, x \notin L -> is_term (t ^ x)) ->
+      is_term (term_lam t)
+  | is_term_app : forall t1 t2,
+      is_term t1 ->
+      is_term t2 ->
+      is_term (term_app t1 t2).
+
+Inductive value : term -> Prop :=
+  | value_lam : forall t, is_term (term_lam t) -> value (term_lam t).
+      
+Inductive step_beta : term -> term -> Prop :=
+  | step_app1 : forall t1 t1' t2,
+      step_beta t1 t1' ->
+      step_beta (term_app t1 t2) (term_app t1' t2)
+  | step_app2 : forall v1 t2 t2',
+      value v1 ->
+      step_beta t2 t2' ->
+      step_beta (term_app v1 t2) (term_app v1 t2')
+  | step_red : forall t v,
+      value v ->
+      is_term t ->
+      step_beta (term_app (term_lam t) v) (t ^^ v).
+
+Notation "t --> t'" := (step_beta t t') (at level 68).
+
+Definition ctx := env type.
+
+Reserved Notation "E |= t ~: T" (at level 69).
+
+Inductive typing : ctx -> term -> type -> Prop :=
+  | typing_var : forall E x T,
+      ok E ->
+      binds x T E ->
+      E |= (term_fvar x) ~: T
+  | typing_lam : forall L E U T t,
+      (forall x, x \notin L ->
+        (E & x ~ U) |= t ^ x ~: T) ->
+      E |= (term_lam t) ~: (type_fun U T)
+  | typing_app : forall S T E t1 t2,
+      E |= t1 ~: (type_fun S T) ->
+      E |= t2 ~: S ->
+      E |= (term_app t1 t2) ~: T
+
+where "E |= t ~: T" := (typing E t T).
+
+Definition preservation_statement := forall E t t' T,
+  E |= t ~: T ->
+  t --> t' ->
+  E |= t' ~: T.
+
+Definition progress_statement := forall t T,
+  empty |= t ~: T ->
+     value t
+  \/ exists t', t --> t'.
+
+Fixpoint fv (t : term) : vars :=
+  match t with
+  | term_bvar i => \{}
+  | term_fvar x => \{x}
+  | term_app lhs rhs => fv lhs \u fv rhs
+  | term_lam body => fv body
+  end.
+
+Fixpoint subst (x : var) (u : term) (t : term) : term :=
+  match t with
+  | term_bvar i => t
+  | term_fvar y => If x = y then u else t
+  | term_app lhs rhs => term_app (subst x u lhs) (subst x u rhs)
+  | term_lam body => term_lam (subst x u body)
+  end.
+
+Notation "[ z ~> u ] t" := (subst z u t) (at level 68).
+
+Ltac gather_vars :=
+  let A := gather_vars_with (fun x : vars => x) in
+  let B := gather_vars_with (fun x : var => \{x}) in
+  let C := gather_vars_with (fun x : ctx => dom x) in
+  let D := gather_vars_with (fun x : term => fv x) in
+  constr:(A \u B \u C \u D).
+
+Ltac pick_fresh x :=
+  let L := gather_vars in (pick_fresh_gen L x).
+Tactic Notation "apply_fresh" constr(T) "as" ident(x) :=
+  apply_fresh_base T gather_vars x.
+Tactic Notation "apply_fresh" "*" constr(T) "as" ident(x) :=
+  apply_fresh T as x; autos*.
+Tactic Notation "apply_fresh" constr(T) :=
+  apply_fresh_base T gather_vars ltac_no_arg.
+Tactic Notation "apply_fresh" "*" constr(T) :=
+  apply_fresh T; auto_star.
+
+Hint Constructors is_term value step_beta.
+
+Axiom subst_open_var : forall x y u t,
+  y <> x -> is_term u ->
+  ([x ~> u]t) ^ y = [x ~> u] (t ^ y).
+
+Axiom subst_intro : forall x t u,
+  x \notin (fv t) -> is_term u ->
+  t ^^ u = [x ~> u](t ^ x).
+
+Local Hint Extern 1 (is_term _) => skip.
+Local Hint Extern 1 (ok _) => skip.
+
+Lemma typing_weaken : forall G E F t T,
+   (E & G) |= t ~: T ->
+   ok (E & F & G) ->
+   (E & F & G) |= t ~: T.
+Proof.
+  introv Typ.
+  (* because of limitations to the [induction] tactic,
+     (limitations not entirely solved by [dependent induction]),
+     we need to manually generalize the parameters of the
+     judgment that we perform the induction on. *)
+  gen_eq H: (E & G). gen G.
+  induction Typ; intros G EQ Ok; subst.
+  apply* typing_var. apply* binds_weaken.
+  (* --begin case abs-- *)
+  (* first we compute [L'], the set of used variables *)
+  let L := gather_vars in sets L': L.
+  (* now we apply [typing_abs] using [L'] *)
+  apply (@typing_lam L').
+  (* we can introduce a name [y] such that [y \notin L'] *)
+  intros y Fry. subst L'.
+  (* to apply the induction hypothesis, we need to rewrite
+     the context for associativity *)
+  rewrite <- concat_assoc.
+  (* now we can apply the induction hypothesis *)
+  apply H0.
+    auto. (* we can prove [y \notin L] *)
+    rewrite concat_assoc. auto.
+    rewrite concat_assoc. auto.
+  (* --end case abs-- *)
+  apply* typing_app.
+Qed.
+
+Lemma typing_subst : forall F E t T z u U,
+  (E & z ~ U & F) |= t ~: T ->
+  E |= u ~: U ->
+  (E & F) |= [z ~> u]t ~: T.
+Proof.
+  introv Typt Typu. gen_eq G: (E & z ~ U & F). gen F.
+  induction Typt; intros G Equ; subst; simpl subst.
+  case_var.
+    binds_get H0. apply_empty* typing_weaken.
+    binds_cases H0; apply* typing_var.
+  apply_fresh typing_lam as y.
+   rewrite* subst_open_var. apply_ih_bind* H0.
+  apply* typing_app.
+Qed.
+
+Lemma preservation_result : preservation_statement.
+Proof.
+  introv Typ. gen t'.
+  induction Typ; intros t' Red; inversions Red.
+  apply* typing_app.
+  apply* typing_app.
+  inversions Typ1. 
+    pick_fresh x. rewrite* (@subst_intro x).
+    apply_empty* typing_subst.
+Qed.
+
+Lemma progress_result : progress_statement.
+Proof.
+  introv Typ. gen_eq E: (empty:ctx). lets Typ': Typ.
+  induction Typ; intros; subst.
+  false* binds_empty_inv.
+  left*.
+  right. destruct~ IHTyp1 as [Val1 | [t1' Red1]].
+    destruct~ IHTyp2 as [Val2 | [t2' Red2]].
+      inversions Typ1; inversions Val1. exists* (t ^^ t2).
+      exists* (term_app t1 t2').
+    exists* (term_app t1' t2).
+Qed.
 
 
-
-Definition ctx := partial_map
-
-(* Inductive typing : ctx -> syntax -> type :=
-  in_ctx :  *)
